Finish refactor to use generic wp_modify rule
All the wprules for get, put, alloc and free now use modifyS and
modifyS' as their underlying abstraction. Making it easer to redo their
proof in the future.

theories/program_logic/state.v
@@ -20,6 +20,10 @@ Instance mbind_state ST: MBind (state ST) :=
                           | None => None
                           end.
 
+
+Definition modifyS' {A ST} (f: ST -> A * ST): state ST A :=
+  State $ λ st, Some $ f st.
+
 Section state_op.
    Context {ST A: Type}.
 
@@ -29,10 +33,13 @@ Section state_op.
    Definition putS (x: ST): state ST unit :=
      State $ λ st, Some (tt, x).
 
+   Definition modifyS (f: ST -> ST): state ST () :=
+     modifyS' $ λ st, (tt, f st).
+
    Definition fail: state ST A :=
      State $ λ st, None.
 
-    Definition ret_fail {S A} (m: option A): state S A := 
+    Definition ret_fail (m: option A): state ST A := 
      match m with
      | Some x => mret x
      | None => fail
@@ -42,23 +49,16 @@ End state_op.
 
 Section gmap_state.
   Definition get {A} (n: nat): state (gmap nat A) A :=
-    State $ λ (st: gmap nat A), (λ x, (x, st)) <$> lookup n st.
-
-  Definition get' {A} (n: nat): state (gmap nat A) A :=
     getS ≫= λ st, ret_fail $ lookup n st.
 
   Definition put {A} (n: nat) (x : A) : state (gmap nat A) unit :=
-    State $ λ st, Some (tt, <[n := x]> st).
-
-  Definition put' {A} (n: nat) (x : A) : state (gmap nat A) unit :=
-    getS ≫= λ st, putS $ <[n := x]> st.
+    modifyS <[n := x]>.
 
   Definition alloc {A} (v: A) : state (gmap nat A) nat :=
-    getS ≫= λ st, 
+    modifyS'$ λ st, 
                 let fresh := fresh $ dom (gset nat) st
-                in putS $ <[fresh := v]> st ;; mret fresh.
+                in (fresh, <[fresh := v]> st). 
 
   Definition free {A} (n: nat): state (gmap nat A) unit :=
-    getS ≫= λ st, putS $ delete n st.
-
+    modifyS $ delete n.
 End gmap_state.
